updated compcerto

compcertox/Composition.v
@@ -1,10 +1,10 @@
 Require Import Relations RelationClasses Relators.
 Require Import List.
 Require Import Coqlib.
-Require Import LanguageInterface Events Globalenvs Smallstep.
+Require Import LanguageInterface_ Events Globalenvs Smallstep_ CategoricalComp.
 Require Import Memory Values.
-Require Import Clight Linking.
-Require Import AbsRel ClightLinking Lifting CatComp.
+Require Import Clight_ Linking.
+Require Import AbstractStateRel Lifting.
 Require Import Maps.
 
 Set Implicit Arguments.
@@ -32,276 +32,44 @@ Notation "R1 ∘ R2" := (vcomp_rel R1 R2): krel_scope.
 
 Coercion absrel_to_cc : rel_adt >-> callconv.
 
-Definition layer_combine {K} (M: Clight.program) (L: layer K) sk :=
-  layer_comp (semantics1 M @ K) L sk.
+(* A module is a list of compilation units. Specifically, they are Clight
+   programs at this time. Note that in the layer library the modules are
+   organized as mapping from identifiers to vars or functions. A module like
+   that is transformed into a Clight program by [make_program] because separate
+   compilation is not supported. However, here a module is nothing but a list of
+   programs and the semantics is given by the horizontal composition of the
+   Clight programs *)
+Definition cmodule := list Clight_.program.
 
+Fixpoint semantics (cmod: cmodule) sk: semantics li_c li_c :=
+  match cmod with
+  | nil => id_semantics sk
+  | (p :: ps) =>
+    let L b := match b with
+               | true =>  semantics ps sk
+               | false => Clight_.semantics1 p
+               end
+    in SmallstepLinking_.semantics L sk
+  end.
 
-(* E@K1    -–M-->    F@K2 *)
+Definition cmod_combine := app.
+Notation " M ⊕ N " := (cmod_combine M N) (left associativity, at level 50).
 
-(*               C_F@K2 *)
-(*                 |    *)
-(*                 R    *)
-(*                 |    *)
-(* C_E@K1 --M--> C_F@K1 *)
+Definition layer_comp {K} (M: cmodule) (L: layer K) sk :=
+  comp_semantics' (semantics M sk @ K) L sk.
 
-(*
-
-  underlay -> (L2 : !E or 1 -> E)
-  strategy -> M (Clight.program) or F (linear map E --o F)
-  overlay -> F o L2
-
-  K1 ~ trace F
-
-  K2 ~ trace E + memory
-
-  M_cnt o L_int
-
-
-  1 |- M_int : L_int
-  L_int |- M_cnt : L_cnt
-------------------------------vcomp
-  1 |- M_int + M_cnt : L_cnt
-
-
-
-
-  counter:  L_cnt <=_R  M_cnt o L_int
-  getter/setter:  L_int <= M_int
-
-*)
-
-Definition prog_ksim {K1 K2: Type} (L1: layer K1)
-           (L2: layer K2) (M: Clight.program) (R: rel_adt K1 K2) :=
-  forall sk, link (skel (semantics1 M)) (skel L2) = Some sk ->
-        forward_simulation 1 R L1 (layer_combine M L2 sk).
-
-Require Import Ctypes.
-
-Lemma link_fundef_lemma {F} (x y z xy xyz: fundef F):
-  link x y = Some xy -> link xy z = Some xyz -> exists yz, link y z = Some yz /\ link x yz = Some xyz.
-Proof.
-  Local Transparent Linker_fundef.
-  intros Hxy Hxyz. inv Hxy. inv Hxyz.
-  unfold link_fundef in *.
-  destruct x eqn: Hx.
-  - destruct y eqn: Hy; try congruence.
-    destruct e eqn: He; try congruence.
-    inv H0.
-    destruct z eqn: Hz; try congruence.
-    destruct e eqn: He'; try congruence.
-    eexists. split. cbn.
-Admitted.
-
-
-Lemma link_def_lemma (x y z xy xyz: AST.globdef unit unit):
-  link x y = Some xy -> link xy z = Some xyz -> exists yz, link y z = Some yz.
-Proof.
-  Local Transparent Linker_unit Linker_def Linker_vardef Linker_varinit.
-  intros Hxy Hxyz. inv Hxy. inv Hxyz.
-Admitted.
-
-Lemma link_prog_lemma (x y z xy xyz: AST.program unit unit):
-  link x y = Some xy -> link xy z = Some xyz -> exists yz, link y z = Some yz /\ link x yz = Some xyz.
-Proof.
-Admitted.
-(* Local Transparent Linker_prog. *)
-(* intros Hxy Hxyz. *)
-(* pose proof (link_linkorder _ _ _ Hxy) as [Hox Hoy]. *)
-(* inv Hxy. inv Hxyz. *)
-(* apply link_prog_inv in H0 as (Ha1 & Hb1 & Hc1). *)
-(* apply link_prog_inv in H1 as (Ha2 & Hb2 & Hc2). *)
-(* eexists. cbn. unfold link_prog. *)
-(* destruct (AST.ident_eq (_ y) (_ z)). *)
-(* 2: { exfalso. rewrite Hc1 in Ha2. cbn in Ha2. congruence. } *)
-(* simpl. destruct (Maps.PTree_Properties.for_all (_ y) _) eqn: Hx; *)
-(*          [reflexivity | exfalso]. *)
-(* rewrite Maps.PTree_Properties.for_all_false in Hx. *)
-(* destruct Hx as (idx & def & Hx & Hy). *)
-(* assert (link_prog_check y z idx def = true). *)
-(* { *)
-(*   clear Hy Hc2. unfold link_prog_check. *)
-(*   rename Hx into Hy. *)
-(*   destruct (Maps.PTree.get idx (_ z)) eqn: Hz; auto. *)
-(*   destruct (Maps.PTree.get idx (AST.prog_defmap x)) eqn: Hx. *)
-(*   - specialize (Hb1 _ _ _ Hx Hy) as (Ha & Hb & Hc). *)
-(*     destruct (in_dec _ _ (_ y)); try congruence; simpl. *)
-(*     pose proof (prog_defmap_linkorder x xy _ _ Hox Hx) as (gxy & Hxy & ?). *)
-(*     specialize (Hb2 _ _ _ Hxy Hz) as (? & ? & ?). *)
-(*     destruct (in_dec _ _ (_ z)); try congruence; simpl. *)
-(*     destruct Hc as (gxy' & Hgxy). *)
-(*     assert (gxy = gxy') as <-. *)
-(*     + admit. *)
-(*     + destruct H2 as (gxyz & Hgxyz). *)
-(*       exploit link_def_lemma. apply Hgxy. eauto. *)
-(*       intros (? & Hgyz). inv Hgyz. rewrite H3. auto. *)
-(*   - admit. *)
-(* (* Whether or not idx is a public definition in y doesn't affect how x and *)
-(*          y are linked. But if it is private in y, xy and z cannot be linked  *) *)
-(* } *)
-(* now rewrite H in Hy. *)
-(* Admitted. *)
-
-Require Import CallconvAlgebra.
-
-(* move to CatComp.v *)
-Definition layer_compose {li} L1 (L2: Smallstep.semantics li_null li) :=
-  option_map (layer_comp L1 L2) (link (skel L1) (skel L2)).
-
-Lemma layer_comp_fsim' {li1 li2} (cc: callconv li1 li2) L1a L1b L1 L2a L2b L2:
-  forward_simulation cc cc L1a L2a ->
-  forward_simulation 1 cc L1b L2b ->
-  layer_compose L1a L1b = Some L1 ->
-  layer_compose L2a L2b = Some L2 ->
-  forward_simulation 1 cc L1 L2.
-Proof.
-Admitted.
-
-Lemma identity_lift_fsim {K liA liB} (L1 L2: Smallstep.semantics liA liB):
-  forward_simulation 1 1 L1 L2 ->
-  forward_simulation 1 1 (L1 @ K) (L2 @ K).
-Proof.
-Admitted.
-
-Lemma lift_composition_fsim {K li} (L1 L2: Smallstep.semantics li li) L:
-  SmallstepLinking.compose L1 L2 = Some L ->
-  exists LK, SmallstepLinking.compose (L1 @ K) (L2 @ K) = Some LK /\
-        forward_simulation 1 1 LK (L @ K).
-Proof.
-Admitted.
-
-Lemma compose_forward_simulations1 {li} (L1 L2 L3: semantics li li):
-  forward_simulation 1 1 L1 L2 -> forward_simulation 1 1 L2 L3 -> forward_simulation 1 1 L1 L3.
-Proof.
-  intros. eapply open_fsim_ccref.
-  apply cc_compose_id_left.
-  apply cc_compose_id_left.
-  eapply compose_forward_simulations; eauto.
-Qed.
-
-Lemma magic_simulation {li} (L1 L2: Smallstep.semantics li li) L3 sk sk1 sk2:
-  let LX := SmallstepLinking.semantics (fun i => match i with true => L1 | false => L2 end) sk1 in
-  let LY := layer_comp L1 (layer_comp L2 L3 sk2) sk in
-  forward_simulation 1 1 LY (layer_comp LX L3 sk).
-Proof.
-Admitted.
-
-(* Lemma magic_simulation' {li K} (L1 L2: Smallstep.semantics li li) L3 LK L12 L23 L123 L123': *)
-(*   SmallstepLinking.compose (L1 @ K) (L2 @ K) = Some L12 -> layer_compose LK L3 = Some L123' -> *)
-(*   layer_compose (L2 @ K) L3 = Some L23 -> layer_compose (L1 @ K) L23 = Some L123 -> *)
-(*   forward_simulation 1 1 L123 L123'. *)
-(* Proof. *)
-(* Admitted. *)
-
-Lemma clight_sim' {K1 K2} (R: rel_adt K1 K2) p:
-  forward_simulation R R (Clight.semantics1 p @ K1) (Clight.semantics1 p @ K2).
-Proof.
-  induction R; simpl.
-  - apply identity_lift_fsim.
-    apply identity_forward_simulation.
-  - apply clight_sim.
-  - eapply compose_forward_simulations; eauto.
-Qed.
-
-Require Import Coq.Logic.FunctionalExtensionality.
-
-Lemma if_commute {A B} x y (f: A -> B):
-  (fun i : bool => f (if i then x else y)) = (fun i : bool => (if i then f x else f y)).
-Proof.
-  apply functional_extensionality.
-  intros i. destruct i; f_equal.
-Qed.
+Definition ksim {K1 K2: Type} (L1: layer K1) (L2: layer K2)
+           (M: cmodule) (R: rel_adt K1 K2) :=
+  forward_simulation 1 R L1 (layer_comp M L2 (skel L1)).
 
 Section VCOMP.
 
-  Context {K1 K2 K3 L1 L2 L3} {M N: Clight.program}
+  Context {K1 K2 K3 L1 L2 L3} {M N: cmodule}
           {R: rel_adt K1 K2} {S: rel_adt K2 K3}
-          (HL1: prog_ksim L1 L2 M R) (HL2: prog_ksim L2 L3 N S).
-  Context (p: Clight.program) (Hp: link M N = Some p).
+          (HL1: ksim L1 L2 M R) (HL2: ksim L2 L3 N S).
 
-  Theorem layer_vcomp: prog_ksim L1 L3 p (R ∘ S).
+  Theorem layer_vcomp: ksim L1 L3 (M ⊕ N) (R ∘ S).
   Proof.
-    intros sk Hsk.
-    assert (Hskp: link (skel (semantics1 M)) (skel (semantics1 N)) = Some (skel (semantics1 p))).
-    {
-      apply link_erase_program.
-      Local Transparent Linker_program.
-      inv Hp. unfold link_program in H0.
-      destruct (link (program_of_program M) (program_of_program N)); try congruence.
-      destruct lift_option; try congruence.
-      destruct s. destruct link_build_composite_env. destruct a.
-      unfold program_of_program. inv H0. cbn. destruct p0. reflexivity.
-    }
-    exploit link_prog_lemma; [ apply Hskp | apply Hsk | ].
-    intros (sk2 & Hsk2 & Hsk1). specialize (HL2 Hsk2). inv HL2. rename X into HL2.
-    exploit HL1. rewrite (fsim_skel HL2). eauto. clear HL1. intros [HL1].
-
-    simpl. exploit @compose_forward_simulations.
-    constructor. apply HL1.
-    2: {
-      intro X. eapply open_fsim_ccref.
-      apply cc_compose_id_left.
-      unfold flip. reflexivity.
-      apply X.
-    }.
-
-    eapply open_fsim_ccref. apply cc_compose_id_left. apply cc_compose_id_right.
-    exploit @lift_composition_fsim. unfold SmallstepLinking.compose.
-    rewrite Hskp. reflexivity.
-    intros (LK & ? & HLK).
-    eapply compose_forward_simulations.
-    2: {
-      assert (HX: layer_compose (semantics1 p @ K3) L3 =
-                  Some (layer_combine p L3 sk)).
-      unfold layer_compose. cbn -[link].
-      cbn -[link] in Hsk. rewrite Hsk. reflexivity.
-
-      eapply layer_comp_fsim';
-        [ | apply identity_forward_simulation | | apply HX ].
-
-      eapply compose_forward_simulations1.
-      2: {
-        apply identity_lift_fsim.
-        apply clight_linking. eauto.
-      }
-      rewrite if_commute. cbn in HLK |- *. apply HLK.
-
-      unfold layer_compose. destruct HLK.
-      rewrite (fsim_skel f). cbn -[link semantics1].
-      rewrite Hsk. reflexivity.
-    } clear HLK.
-
-    pose proof (magic_simulation (semantics1 M @ K3) (semantics1 N @ K3) L3 sk (AST.erase_program p) sk2) as X.
-    cbn in X. unfold SmallstepLinking.compose in H. cbn in Hskp, H. rewrite Hskp in H. cbn in H.
-    injection H. intros Hr. rewrite Hr in X. clear H.
-    (* exploit @magic_simulation; [ apply H0 | ..]. *)
-    (* { *)
-    (*   instantiate (2 := L3). instantiate (2 := LK). *)
-    (*   unfold SmallstepLinking.compose in H0. *)
-    (*   Opaque Linker_prog. *)
-    (*   cbn in H', H0. rewrite H' in H0. cbn in H0. *)
-    (*   unfold layer_compose. injection H0. intros Hk. *)
-    (*   rewrite <- Hk at 2. cbn in Hsk |- *. rewrite Hsk. reflexivity. *)
-    (* } *)
-    (* { *)
-    (*   unfold layer_compose. cbn in Hsk2 |- *. rewrite Hsk2. reflexivity. *)
-    (* } *)
-    (* { *)
-    (*   unfold layer_compose. cbn. inv HL2. rewrite (fsim_skel X) in *. *)
-    (*   cbn in Hsk1 |- *. rewrite Hsk1. reflexivity. *)
-    (* } *)
-    (* intros X. *)
-
-    eapply open_fsim_ccref. apply cc_compose_id_left. apply cc_compose_id_right.
-    eapply compose_forward_simulations; [ | apply X ].
-    eapply layer_comp_fsim'; [ | constructor; apply HL2 | ..].
-    (* instantiate (1 := ((semantics1 M) @ K3)%sem). *)
-    (* instantiate (1 := ((semantics1 M) @ K2)%sem). *)
-    apply clight_sim'.
-    unfold layer_compose. rewrite (fsim_skel HL2). cbn in Hsk1 |- *. rewrite Hsk1. reflexivity.
-    unfold layer_combine, layer_compose.
-    cbn in Hsk1 |- *. rewrite Hsk1. reflexivity.
-  Qed.
+  Admitted.
 
 End VCOMP.
-
-Require Import FlatComp.
